src/ModSim.v
@@ -1420,6 +1420,19 @@ Section PRIMIVIESIM.
                   (ths, im_src1, im_tgt3, st_src2, st_tgt2)
                   >>)).
 
+  Definition local_sim_init {R0 R1} (RR: R0 -> R1 -> Prop) (r_own: URA.car) tid src tgt :=
+    forall ths im_src im_tgt st_src st_tgt r_shared r_ctx
+           (INV: I (ths, im_src, im_tgt, st_src, st_tgt) r_shared)
+           (VALID: URA.wf (r_shared ⋅ r_own ⋅ r_ctx)),
+    forall im_tgt1 (FAIR: fair_update im_tgt im_tgt1 (sum_fmap_l (tids_fmap tid ths))),
+    forall fs ft,
+      lsim
+        tid
+        (@local_RR R0 R1 RR tid)
+        fs ft
+        r_ctx
+        src tgt
+        (ths, im_src, im_tgt1, st_src, st_tgt).
 End PRIMIVIESIM.
 #[export] Hint Constructors __lsim: core.
 #[export] Hint Unfold lsim: core.
@@ -1427,6 +1440,38 @@ End PRIMIVIESIM.
 #[export] Hint Resolve _lsim_mon: paco.
 #[export] Hint Resolve lsim_mon: paco.
 #[export] Hint Resolve cpn9_wcompat: paco.
+
+
+Require Import List.
+From Fairness Require Import Concurrency.
+
+Module UserSim.
+  Section MODSIM.
+
+    Variable md_src: Mod.t.
+    Variable md_tgt: Mod.t.
+
+    Record sim (p_src: Th.t _) (p_tgt: Th.t _) : Prop :=
+      mk {
+          wf_src : WF;
+          wf_tgt : WF;
+          wf_tgt_inhabited: inhabited wf_tgt.(T);
+          wf_tgt_open: forall (o0: wf_tgt.(T)), exists o1, wf_tgt.(lt) o0 o1;
+
+          world: URA.t;
+
+          funs: forall im_tgt,
+          exists im_src rs r_shared I,
+            (<<INIT: I (key_set p_src, im_src, im_tgt, md_src.(Mod.st_init), md_tgt.(Mod.st_init)) r_shared>>) /\
+              (<<SIM: Forall3
+                        (fun '(t1, src) '(t2, tgt) '(t3, r) =>
+                           (t1 = t2 /\ t1 = t3) /\
+                           @local_sim_init _ md_src.(Mod.state) md_tgt.(Mod.state) md_src.(Mod.ident) md_tgt.(Mod.ident) wf_src wf_tgt I _ _ (@eq Any.t) r t1 src tgt)
+                        (Th.elements p_src) (Th.elements p_tgt) (NatMap.elements rs)>>) /\
+              (<<WF: URA.wf (r_shared ⋅ NatMap.fold (fun _ r s => r ⋅ s) rs ε)>>)
+        }.
+  End MODSIM.
+End UserSim.
 
 
 Module ModSim.
